src/GoExtraction.v
@@ -42,17 +42,21 @@ Ltac source_stmt_step :=
 Ltac find_val v p :=
   match p with
     | context[?k ~> v] => constr:(Some k)
+    (* TODO: more principled thing? *)
+    | context[?k |-> Val _ (id v)] => constr:(Some k)
     | _ => constr:(@None var)
   end.
 
 Ltac find_val_fn v p cont :=
   match p with
     | context[?k ~> v] => cont k
+    | context[?k |-> Val _ (id v)] => cont k
   end.
 
 Ltac var_mapping_to pred val :=
   lazymatch pred with
     | context[?var ~> val] => var
+    | context[?var |-> Val _ (id val)] => var
   end.
 
 Definition mark_ret (T : Type) := T.
@@ -155,7 +159,7 @@ Ltac compile_ret :=
       match var_mapping_to_ret with
       | ?kret => (unify kx kret; fail 2) ||
                                         eapply hoare_weaken; [
-                  eapply CompileDup with (var0 := kx) (var' := kret)
+                  eapply CompileMove with (var0 := kx) (var' := kret)
                 | cancel_go.. ]
       end
     end
@@ -277,22 +281,13 @@ Ltac get_head E :=
   | ?P => constr:(P)
   end.
 
-Ltac ensure_val_has_dup_and_get val_ cont :=
+Ltac ensure_val_present val_ cont :=
   let T := type of val_ in
   lazymatch goal with
   |- EXTRACT _ {{ ?pre_ }} _ {{ _ }} // _ =>
-    lazymatch pre_ with
-    | context [?k1 ~> val_] =>
-      match pre_ with
-      | context [?k2 ~> val_ ] =>
-        try (unify k1 k2; fail 1); cont k2
-      | _ =>
-        do_declare T ltac:(fun var =>
-          eapply hoare_weaken; [
-          eapply SetVarBefore with (val := val_) (var0 := var) | cancel_go..]
-        )
-      end
-    | _ => do_declare T ltac:(fun var =>
+    match find_val val_ pre_ with
+    | Some ?k1 => cont k1
+    | None => do_declare T ltac:(fun var =>
           eapply hoare_weaken; [
           eapply SetVarBefore with (val := val_) (var0 := var) | cancel_go..]
         )
@@ -301,7 +296,7 @@ Ltac ensure_val_has_dup_and_get val_ cont :=
 
 Ltac declare_and_get_args' expr argvars cont :=
   lazymatch expr with
-  | ?rest ?arg => ensure_val_has_dup_and_get arg ltac:(fun var_ => declare_and_get_args' rest (var_, argvars) cont)
+  | ?rest ?arg => ensure_val_present arg ltac:(fun var_ => declare_and_get_args' rest (var_, argvars) cont)
   | ?f => cont argvars
   end.
   
